theories/SpecNotations.v
@@ -8,5 +8,3 @@ Notation "⊢ v 'in' t" := (Jv v t) (at level 90).
 Notation "v0 ⇓ v1" := (big v0 v1) (at level 90).
 
 Notation "Δ ⊢ E [ v ]" := (sat Δ E v) (at level 90).
-
-Notation "[ x := E ]" := (subst_context E x).
